theories/Interp/Handler.v
@@ -1,7 +1,7 @@
-(** * Effect handlers *)
+(** * Event handlers *)
 
-(** Effects [E, F : Type -> Type] and itree [E ~> itree F] form a
-    category. *)
+(** Events types [E, F : Type -> Type] and itree [E ~> itree F]
+    form a category. *)
 
 (* begin hide *)
 From Coq Require Import
@@ -29,36 +29,37 @@ Open Scope itree_scope.
 
 Module Handler.
 
-(** Lift an _effect morphism_ into an _effect handler_. *)
-Definition hsend {A B} (m : A ~> B) : A ~> itree B :=
-  fun _ e => ITree.send (m _ e).
+(** Lift an _event morphism_ into an _event handler_. *)
+Definition htrigger {A B} (m : A ~> B) : A ~> itree B :=
+  fun _ e => ITree.trigger (m _ e).
 
-(** This handler just wraps effects back into itrees, which is
-    a noop (modulo taus): [interp (id_ E) _ t ≈ t]. *)
-Definition id_ (E : Type -> Type) : E ~> itree E := ITree.send.
+(** Trivial handler, triggering any event it's given, so
+    the resulting interpretation is the identity function:
+    [interp (id_ E) _ t ≈ t]. *)
+Definition id_ (E : Type -> Type) : E ~> itree E := ITree.trigger.
 
-(** Chain handlers: [g] handles the effects produced by [f]. *)
+(** Chain handlers: [g] handles the events produced by [f]. *)
 Definition cat {E F G : Type -> Type}
            (f : E ~> itree F) (g : F ~> itree G)
   : E ~> itree G
   := fun R e => interp g (f R e).
 
-(** Wrap effects to the left of a sum. *)
+(** Wrap events to the left of a sum. *)
 Definition inl_ {E F : Type -> Type} : E ~> itree (E +' F)
-  := hsend inl1.
+  := htrigger inl1.
 
-(** Wrap effects to the right of a sum. *)
+(** Wrap events to the right of a sum. *)
 Definition inr_ {E F : Type -> Type} : F ~> itree (E +' F)
-  := hsend inr1.
+  := htrigger inr1.
 
-(** Case analysis on sums of effects. *)
+(** Case analysis on sums of events. *)
 Definition case_ {E F G : Type -> Type}
            (f : E ~> itree G) (g : F ~> itree G)
   : E +' F ~> itree G
   := @case_sum1 E F (itree G) f g.
 (* TODO: why is there a universe inconsistency if this is before [inl_] and [inr_]? *)
 
-(** Handle independent effects. *)
+(** Handle events independently, with disjoint sets of output events. *)
 Definition bimap {E F G H : Type -> Type}
            (f : E ~> itree G) (g : F ~> itree H)
   : E +' F ~> itree (G +' H)
