theories/Events/Dependent.v
@@ -1,4 +1,4 @@
-(** * Dependently-typed effects *)
+(** * Dependently-typed events *)
 
 (** A _type family_ is given by a parameter type [I : Type] and a type function
     [F : I -> Type].
@@ -8,7 +8,9 @@
     A value [i : I] can be seen as a "flat representation" of a value [e : E X]
     (for arbitrary [X]), while [F i : Type] gives the type index [X] of this [e].
 
-    This encoding can be seen as a kind of "dependently-typed effect".
+    This encoding can be seen as a kind of "dependently-typed event",
+    although the general use indexed types for event types already provides an
+    equally expressive form of dependency.
  *)
 
 (* begin hide *)
@@ -16,7 +18,7 @@ From ITree Require Import
      Basics.Basics
      Core.ITreeDefinition
      Indexed.Sum
-     Indexed.OpenSum.
+     Core.Subevent.
 
 Import Basics.Basics.Monads.
 (* end hide *)
@@ -27,7 +29,7 @@ Variant depE {I : Type} (F : I -> Type) : Type -> Type :=
 Arguments Dep {I F}.
 
 Definition dep {I F E} `{depE F -< E} (i : I) : itree E (F i) :=
-  send (Dep i).
+  trigger (Dep i).
 
 Definition undep {I F} (f : forall i : I, F i) :
   depE F ~> identity :=
