theories/Interp/HandlerFacts.v
@@ -35,7 +35,7 @@ Instance CatIdL_Handler : CatIdL Handler.
 Proof.
   red; intros A B f X e.
   unfold cat, Cat_Handler, Handler.cat, id_, Id_Handler, Handler.id_.
-  rewrite interp_send, tau_eutt.
+  rewrite interp_trigger, tau_eutt.
   reflexivity.
 Qed.
 
